First_Order_Clause: Polymorphic Ground Terms

thys/First_Order_Clause/IsaFoR_Ground_Term.thy
@@ -1,183 +1,21 @@
 theory IsaFoR_Ground_Term
   imports 
     "Regular_Tree_Relations.Ground_Terms"
-    Parallel_Induct
+    Generic_Term
 begin
 
-type_synonym 'f ground_term = "'f gterm"
- 
-no_notation Sublist.parallel (infixl \<open>\<bottom>\<close> 64)
+abbreviation (input) is_var where
+  "is_var _ \<equiv> False"
 
-(* TODO: Generalize consts for abstract contexts *)
-abbreviation positions\<^sub>G where
-  "positions\<^sub>G \<equiv> gposs"
+interpretation gterm: smaller_subterms where
+  subterms = gargs and size = size and is_var = is_var
+  by 
+    unfold_locales
+    (metis add.commute elem_size_size_list_size gterm.exhaust_sel gterm.size(2) trans_less_add2)
 
-notation gsubt_at (infixl \<open>!\<^sub>t\<^sub>G\<close> 64)
-
-lemma parallel_induct_first_in_positions\<^sub>G [case_names parallel p\<^sub>1_in_t base step]: 
-  assumes
-    parallel: "p\<^sub>1 \<bottom> p\<^sub>2" and
-    p\<^sub>1_in_t: "p\<^sub>1 \<in> positions\<^sub>G t" and
-    base: 
-      "\<And>p\<^sub>1 p\<^sub>2 i j q\<^sub>1 q\<^sub>2 t f ts.
-        p\<^sub>1 = i # q\<^sub>1 \<Longrightarrow> 
-        p\<^sub>2 = j # q\<^sub>2 \<Longrightarrow>
-        i \<noteq> j \<Longrightarrow>
-        t = GFun f ts \<Longrightarrow>
-        i < length ts \<Longrightarrow> P p\<^sub>1 p\<^sub>2 t" and
-    step: 
-      "\<And>p\<^sub>1 p\<^sub>2 p k i j q\<^sub>1 q\<^sub>2 t f ts.
-        p\<^sub>1 = k # p @ i # q\<^sub>1 \<Longrightarrow>
-        p\<^sub>2 = k # p @ j # q\<^sub>2 \<Longrightarrow>
-        i \<noteq> j \<Longrightarrow>
-        t = GFun f ts \<Longrightarrow> 
-        k < length ts \<Longrightarrow>
-        p\<^sub>1 \<in> positions\<^sub>G t \<Longrightarrow>
-        P (p @ i # q\<^sub>1) (p @ j # q\<^sub>2) (ts ! k) \<Longrightarrow>
-        P p\<^sub>1 p\<^sub>2 t"
-    shows "P p\<^sub>1 p\<^sub>2 t"
-  using p\<^sub>1_in_t
-proof (induction arbitrary: t rule: parallel_induct[OF parallel])
-  case base': (1 p\<^sub>1 p\<^sub>2 i j q\<^sub>1 q\<^sub>2 t)
-
-  then obtain f ts where "t = GFun f ts" "i < length ts"
-    by (cases t, auto)
-
-  then show ?case
-    using base' base
-    by metis
-next
-  case step': (2 p\<^sub>1 p\<^sub>2 p k i j q\<^sub>1 q\<^sub>2 t)
-
-  then obtain f ts where t: "t = GFun f ts" and k: "k < length ts" 
-    by (cases t, auto)
-
-  show ?case
-  proof (rule step[OF step'(1, 2, 3) t k step'(5)])
-
-    let ?p\<^sub>1 = "p @ i # q\<^sub>1"
-    let ?p\<^sub>2 = "p @ j # q\<^sub>2" 
-
-    from step' have "?p\<^sub>1 \<in> positions\<^sub>G (ts ! k)"
-      unfolding t
-      by simp
-
-    then show "P ?p\<^sub>1 ?p\<^sub>2 (ts ! k)"
-      using step'.IH
-      by blast
-  qed
-qed
-
-lemma parallel_induct_second_in_positions\<^sub>G [case_names parallel p\<^sub>2_in_t base step]: 
-  assumes
-    parallel: "p\<^sub>1 \<bottom> p\<^sub>2" and
-    p\<^sub>2_in_t: "p\<^sub>2 \<in> positions\<^sub>G t" and
-    base: 
-      "\<And>p\<^sub>1 p\<^sub>2 i j q\<^sub>1 q\<^sub>2 t f ts.
-        p\<^sub>1 = i # q\<^sub>1 \<Longrightarrow> 
-        p\<^sub>2 = j # q\<^sub>2 \<Longrightarrow>
-        i \<noteq> j \<Longrightarrow>
-        t = GFun f ts \<Longrightarrow>
-        j < length ts \<Longrightarrow> P p\<^sub>1 p\<^sub>2 t" and
-    step: 
-      "\<And>p\<^sub>1 p\<^sub>2 p k i j q\<^sub>1 q\<^sub>2 t f ts.
-        p\<^sub>1 = k # p @ i # q\<^sub>1 \<Longrightarrow>
-        p\<^sub>2 = k # p @ j # q\<^sub>2 \<Longrightarrow>
-        i \<noteq> j \<Longrightarrow>
-        t = GFun f ts \<Longrightarrow> 
-        k < length ts \<Longrightarrow>
-        p\<^sub>2 \<in> positions\<^sub>G t \<Longrightarrow>
-        P (p @ i # q\<^sub>1) (p @ j # q\<^sub>2) (ts ! k) \<Longrightarrow>
-        P p\<^sub>1 p\<^sub>2 t"
-    shows "P p\<^sub>1 p\<^sub>2 t"
-  using p\<^sub>2_in_t
-proof (induction arbitrary: t rule: parallel_induct[OF parallel])
-  case base': (1 p\<^sub>1 p\<^sub>2 i j q\<^sub>1 q\<^sub>2 t)
-
-  then obtain f ts where "t = GFun f ts" "j < length ts"
-    by (cases t, auto)
-
-  then show ?case
-    using base' base
-    by metis
-next
-  case step': (2 p\<^sub>1 p\<^sub>2 p k i j q\<^sub>1 q\<^sub>2 t)
-
-  then obtain f ts where t: "t = GFun f ts" and k: "k < length ts" 
-    by (cases t, auto)
-
-  show ?case
-  proof (rule step[OF step'(1, 2, 3) t k step'(5)])
-
-    let ?p\<^sub>1 = "p @ i # q\<^sub>1"
-    let ?p\<^sub>2 = "p @ j # q\<^sub>2" 
-
-    from step' have "?p\<^sub>2 \<in> positions\<^sub>G (ts ! k)"
-      unfolding t
-      by simp
-
-    then show "P ?p\<^sub>1 ?p\<^sub>2 (ts ! k)"
-      using step'.IH
-      by blast
-  qed
-qed
-
-lemma parallel_induct_in_positions\<^sub>G [case_names parallel p\<^sub>1_in_t p\<^sub>2_in_t base step]: 
-  assumes
-    parallel: "p\<^sub>1 \<bottom> p\<^sub>2" and
-    p\<^sub>1_in_t: "p\<^sub>1 \<in> positions\<^sub>G t" and
-    p\<^sub>2_in_t: "p\<^sub>2 \<in> positions\<^sub>G t" and
-    base: 
-      "\<And>p\<^sub>1 p\<^sub>2 i j q\<^sub>1 q\<^sub>2 t f ts.
-        p\<^sub>1 = i # q\<^sub>1 \<Longrightarrow> 
-        p\<^sub>2 = j # q\<^sub>2 \<Longrightarrow>
-        i \<noteq> j \<Longrightarrow>
-        t = GFun f ts \<Longrightarrow>
-        j < length ts \<Longrightarrow>
-        i < length ts \<Longrightarrow>
-        P p\<^sub>1 p\<^sub>2 t" and
-    step: 
-      "\<And>p\<^sub>1 p\<^sub>2 p k i j q\<^sub>1 q\<^sub>2 t f ts.
-        p\<^sub>1 = k # p @ i # q\<^sub>1 \<Longrightarrow>
-        p\<^sub>2 = k # p @ j # q\<^sub>2 \<Longrightarrow>
-        i \<noteq> j \<Longrightarrow>
-        t = GFun f ts \<Longrightarrow> 
-        k < length ts \<Longrightarrow>
-        p\<^sub>1 \<in> positions\<^sub>G t \<Longrightarrow>
-        p\<^sub>2 \<in> positions\<^sub>G t \<Longrightarrow>
-        P (p @ i # q\<^sub>1) (p @ j # q\<^sub>2) (ts ! k) \<Longrightarrow>
-        P p\<^sub>1 p\<^sub>2 t"
-    shows "P p\<^sub>1 p\<^sub>2 t"
-  using p\<^sub>1_in_t p\<^sub>2_in_t
-proof (induction arbitrary: t rule: parallel_induct[OF parallel])
-  case base': (1 p\<^sub>1 p\<^sub>2 i j q\<^sub>1 q\<^sub>2 t)
-
-  then obtain f ts where "t = GFun f ts" "j < length ts" "i < length ts"
-    by (cases t, auto)
-
-  then show ?case
-    using base' base
-    by metis
-next
-  case step': (2 p\<^sub>1 p\<^sub>2 p k i j q\<^sub>1 q\<^sub>2 t)
-
-  then obtain f ts where t: "t = GFun f ts" and k: "k < length ts" 
-    by (cases t, auto)
-
-  show ?case
-  proof (rule step[OF step'(1, 2, 3) t k step'(5, 6)])
-
-    let ?p\<^sub>1 = "p @ i # q\<^sub>1"
-    let ?p\<^sub>2 = "p @ j # q\<^sub>2" 
-
-    from step' have "?p\<^sub>1 \<in> positions\<^sub>G (ts ! k)" "?p\<^sub>2 \<in> positions\<^sub>G (ts ! k)"
-      unfolding t
-      by simp_all
-
-    then show "P ?p\<^sub>1 ?p\<^sub>2 (ts ! k)"
-      using step'.IH
-      by blast
-  qed
-qed
+interpretation gterm: term_interpretation where
+  Fun = "\<lambda>f _. GFun f" and fun_sym = groot_sym and subterms = gargs and extra = "\<lambda>_.()" and
+  is_var = is_var
+  by unfold_locales (auto intro: gterm.exhaust)
 
 end
