thys/First_Order_Clause/Abstract_Context.thy
@@ -1,0 +1,117 @@
+theory Abstract_Context
+  imports Generic_Term_Context
+begin
+
+datatype ('f, 'extra, 't) "context" =
+  Hole (\<open>\<box>\<close>) |
+  More
+    (fun_sym: 'f) (extra: 'extra) (subterms\<^sub>l: "'t list") 
+    (subcontext: "('f, 'extra, 't) context") (subterms\<^sub>r: "'t list")
+
+primrec compose_context (infixl \<open>\<circ>\<^sub>c\<close> 75) where
+  "Hole \<circ>\<^sub>c c = c"
+| "More f e ls C rs \<circ>\<^sub>c D = More f e ls (C \<circ>\<^sub>c D) rs"
+
+fun hole_position :: "('f, 'extra, 't) context \<Rightarrow> position" where
+  "hole_position \<box> = []"
+| "hole_position (More _  _ ss D _) = length ss # hole_position D"
+
+interpretation abstract_context: smaller_subcontext where
+  hole = \<box> and size = size and subcontext = subcontext
+proof unfold_locales
+  fix c :: "('f, 'extra, 't) context"
+  assume "c \<noteq> \<box>"
+
+  then show "size (subcontext c) < size c"
+    by (cases c) auto
+qed
+
+locale abstract_context = 
+  term_interpretation where Fun = Fun +
+  smaller_subterms 
+for Fun :: "'f \<Rightarrow> 'e \<Rightarrow> 't list \<Rightarrow> 't"
+begin
+
+primrec apply_context (\<open>_\<langle>_\<rangle>\<close> [1000, 0] 1000) where
+  "\<box>\<langle>t\<rangle> = t"
+| "(More f e ls C rs)\<langle>t\<rangle> = Fun f e (ls @ C\<langle>t\<rangle> # rs)"
+
+primrec context_at :: "'t \<Rightarrow> position \<Rightarrow> ('f, 'e, 't) context" (infixl \<open>!\<^sub>c\<close> 64) where
+  "t !\<^sub>c [] = \<box>"
+| "t !\<^sub>c i # ps =
+   More
+    (fun_sym t)
+    (extra t)
+    (take i (subterms t)) (subterms t ! i !\<^sub>c ps)
+    (drop (Suc i) (subterms t))"
+
+sublocale "context" where
+  hole = \<box> and 
+  apply_context = apply_context and 
+  compose_context = compose_context
+proof unfold_locales
+  fix c c' t
+
+  show "(c \<circ>\<^sub>c c')\<langle>t\<rangle> = c\<langle>c'\<langle>t\<rangle>\<rangle>"
+    by (induction c) auto
+next
+  fix t
+
+  show "\<box>\<langle>t\<rangle> = t"
+    by simp
+next
+  fix c t t'
+  assume "c\<langle>t\<rangle> = c\<langle>t'\<rangle>"
+
+  then show "t = t'"
+  proof(induction c)
+    case Hole
+    then show ?case
+      by simp
+  next
+    case (More f e ls c rs)
+    then show ?case 
+      by (metis apply_context.simps(2) nth_append_length subterms)
+  qed
+next
+  fix c :: "('f, 'extra, 't) context"
+  show "c \<circ>\<^sub>c \<box> = c"
+    by (induction c) auto
+qed auto
+
+sublocale term_context_interpretation where
+  hole = \<box> and apply_context = apply_context and compose_context = "(\<circ>\<^sub>c)" and
+  More = More and fun_sym\<^sub>c = context.fun_sym and extra\<^sub>c = context.extra and subterms\<^sub>l = subterms\<^sub>l and
+  subcontext = subcontext and subterms\<^sub>r = subterms\<^sub>r 
+proof unfold_locales
+  fix c :: "('f, 'e, 't) context"
+
+  show "c \<noteq> \<box> \<longleftrightarrow> (\<exists>f e ls c' rs. c = More f e ls c' rs)"
+    by (metis context.discI context.exhaust_sel)
+qed auto
+
+interpretation ground_context: replace_at_subterm where  
+  hole = \<box> and apply_context = apply_context and compose_context = "(\<circ>\<^sub>c)" and
+  hole_position = hole_position and context_at = context_at
+proof unfold_locales
+  fix c :: "('f, 'e, 't) context" and t
+
+  show "c\<langle>t\<rangle> !\<^sub>t hole_position c = t"
+    by (induction c) auto
+
+  show "hole_position c \<in> positions c\<langle>t\<rangle>"
+    by (induction c) (auto simp: term_destruct)
+
+  show "c\<langle>t\<rangle> !\<^sub>c hole_position c = c"
+    by (induction c) auto
+next
+  fix p and t
+  assume "p \<in> positions t"
+
+  then show "(t !\<^sub>c p)\<langle>t !\<^sub>t p\<rangle> = t"
+  by (induction p arbitrary: t) (auto simp: Cons_nth_drop_Suc)
+qed auto
+
+end
+
+end
