thys/First_Order_Clause/Generic_Term.thy
@@ -1,0 +1,77 @@
+theory Generic_Term
+  imports Main
+begin
+
+type_synonym position = "nat list"
+
+locale subterms = 
+  fixes subterms :: "'t \<Rightarrow> 't list"
+begin
+
+primrec subterm_at :: "'t \<Rightarrow> position \<Rightarrow> 't" (infixl \<open>!\<^sub>t\<close> 64) where
+  "t !\<^sub>t [] = t" 
+| "t !\<^sub>t i # p = subterms t ! i !\<^sub>t p"
+
+end
+
+locale smaller_subterms = subterms where subterms = subterms 
+  for subterms :: "'t \<Rightarrow> 't list" +
+  notes conj_cong [fundef_cong]
+  fixes size  :: "'t \<Rightarrow> nat" and is_var :: "'t \<Rightarrow> bool"
+  assumes subterms_smaller: "\<And>t' t. t' \<in> set (subterms t) \<Longrightarrow> size t' < size t"
+begin
+
+function positions :: "'t \<Rightarrow> position set" where
+  "positions t =
+     {[]} \<union> {i # p | i p.
+              \<not>is_var t \<and>
+              i < length (subterms t) \<and>
+              p \<in> positions ((subterms t) ! i)}"
+  by pat_completeness auto
+
+termination
+proof (relation "measure size")
+  fix t p i p'
+  assume "p = i # p'" "i < length (subterms t)"
+
+  then show "(subterms t ! i, t) \<in> measure size"
+    using subterms_smaller
+    by simp  
+qed auto
+
+declare positions.simps [simp del]
+
+lemma empty_positions [simp]: "[] \<in> positions t"
+  by (subst positions.simps) blast
+
+lemma nonempty_positions [simp]:
+  "i # p \<in> positions t \<longleftrightarrow> \<not>is_var t \<and> i < length (subterms t) \<and> p \<in> positions ((subterms t) ! i)"
+  by (subst positions.simps) auto
+
+end
+
+locale term_interpretation = 
+  subterms where subterms = subterms
+for subterms :: "'t \<Rightarrow> 't list" +
+fixes 
+  Fun :: "'f \<Rightarrow> 'e \<Rightarrow> 't list \<Rightarrow> 't" and
+  fun_sym :: "'t \<Rightarrow> 'f" and 
+  extra :: "'t \<Rightarrow> 'e" and
+  is_var :: "'t \<Rightarrow> bool"
+assumes
+  term_fun_sym [simp]: "\<And>f e ts. fun_sym (Fun f e ts) = f" and
+  term_extra [simp]: "\<And>f e ts. extra (Fun f e ts) = e" and
+  subterms [simp]: "\<And>f e ts. subterms (Fun f e ts) = ts" and
+  term_destruct: "\<And>t. \<not>is_var t \<longleftrightarrow> (\<exists>f e ts. t = Fun f e ts)" and
+  term_inject [intro]:
+    "\<And>f\<^sub>1 e\<^sub>1 ts\<^sub>1 f\<^sub>2 e\<^sub>2 ts\<^sub>2. Fun f\<^sub>1 e\<^sub>1 ts\<^sub>1 = Fun f\<^sub>2 e\<^sub>2 ts\<^sub>2 \<Longrightarrow> f\<^sub>1 = f\<^sub>2 \<and> e\<^sub>1 = e\<^sub>2 \<and> ts\<^sub>1 = ts\<^sub>2"
+begin
+
+lemma interpret_term [simp]: 
+  assumes "\<not>is_var t"
+  shows "Fun (fun_sym t) (extra t) (subterms t) = t"
+  by (metis assms subterms term_destruct term_extra term_fun_sym)
+
+end
+
+end
