thys/First_Order_Clause/Generic_Term_Context.thy
@@ -1,0 +1,55 @@
+theory Generic_Term_Context
+  imports 
+    Generic_Term
+    Generic_Context
+begin
+
+locale term_context_interpretation = 
+  term_interpretation where Fun = Fun +
+  context_interpretation where More = More and fun_sym = fun_sym\<^sub>c and extra = extra\<^sub>c
+for
+  Fun :: "'f \<Rightarrow> 'e \<Rightarrow> 't list \<Rightarrow> 't" and
+  More :: "'f \<Rightarrow> 'e \<Rightarrow> 't list \<Rightarrow> 'c \<Rightarrow> 't list \<Rightarrow> 'c" and
+  fun_sym\<^sub>c extra\<^sub>c +
+assumes apply_context [simp]: "\<And>f e ls c rs t. (More f e ls c rs)\<langle>t\<rangle> = Fun f e (ls @ c\<langle>t\<rangle> # rs)"
+
+locale hole_position =
+  smaller_subterms where subterms = subterms +
+  "context" where apply_context = apply_context
+for 
+  subterms :: "'t \<Rightarrow> 't list" and
+  apply_context :: "'c \<Rightarrow> 't \<Rightarrow> 't" +
+fixes hole_position :: "'c \<Rightarrow> position"
+assumes 
+  subterm_at_hole_position [simp]: "\<And>c t. c\<langle>t\<rangle> !\<^sub>t hole_position c = t" and
+  hole_position_in_positions [intro]: "\<And>c t. hole_position c \<in> positions (c\<langle>t\<rangle>)"
+
+locale context_at = hole_position where apply_context = apply_context 
+  for apply_context :: "'c \<Rightarrow> 't \<Rightarrow> 't" +
+  fixes context_at :: "'t \<Rightarrow> position \<Rightarrow> 'c" (infixl \<open>!\<^sub>c\<close> 64)
+  assumes
+    context_at_root [simp]: "t !\<^sub>c [] = \<box>" and
+    context_at_hole [simp]: "\<And>c t. c\<langle>t\<rangle> !\<^sub>c (hole_position c) = c" and
+    context_at_subterm_at [simp]: "\<And>p t. p \<in> positions t \<Longrightarrow> (t !\<^sub>c p)\<langle>t !\<^sub>t p\<rangle> = t"
+begin
+
+abbreviation replace_at (\<open>_\<lbrakk>_ := _\<rbrakk>\<close> [70, 0, 50] 70) where
+  "replace_at t p s \<equiv> (t !\<^sub>c p)\<langle>s\<rangle>"
+
+lemma replace_at_hole [simp]: "c\<langle>t\<rangle>\<lbrakk>hole_position c := t'\<rbrakk> = c\<langle>t'\<rangle>"
+  by simp
+
+lemma replace_at_id [simp]: "t\<lbrakk>[] := t\<rbrakk> = t"
+  by simp
+
+end
+
+locale replace_at_subterm = 
+  context_at + 
+  term_interpretation +
+  assumes
+    replace_at_subterm [simp]: 
+      "\<And>f e ts i p t. Fun f e ts\<lbrakk>i # p := t\<rbrakk> =
+        Fun f e (take i ts @ ts ! i\<lbrakk>p := t\<rbrakk> # drop (Suc i) ts)"
+
+end
