thys/First_Order_Clause/IsaFoR_Abstract_Context.thy
@@ -1,0 +1,29 @@
+theory IsaFoR_Abstract_Context
+  imports 
+    First_Order_Terms.Subterm_and_Context
+    Generic_Context
+begin
+
+fun fun_sym\<^sub>c :: "('f, 't) actxt \<Rightarrow> 'f" where
+  "fun_sym\<^sub>c (More f _ _ _) = f"
+
+fun subterms\<^sub>l :: "('f, 't) actxt \<Rightarrow> 't list" where
+  "subterms\<^sub>l (More _ ls _ _) = ls"
+
+fun subcontext :: "('f, 't) actxt \<Rightarrow> ('f, 't) actxt" where
+  "subcontext (More _ _ c _) = c"
+
+fun subterms\<^sub>r :: "('f, 't) actxt \<Rightarrow> 't list" where
+  "subterms\<^sub>r (More _ _ _ rs) = rs"
+
+interpretation abstract_context: smaller_subcontext where
+  hole = \<box> and subcontext = subcontext and size = size
+proof unfold_locales
+  fix c :: "('f, 't) actxt"
+  assume "c \<noteq> \<box>"
+
+  then show "size (subcontext c) < size c"
+    by (cases c) auto
+qed
+
+end
