thys/First_Order_Clause/IsaFoR_Nonground_Term.thy
@@ -1,6 +1,7 @@
 theory IsaFoR_Nonground_Term
   imports 
     Nonground_Term
+    Generic_Term
     Abstract_Substitution.Substitution_First_Order_Term
 begin
 
@@ -10,5 +11,9 @@ global_interpretation "term": nonground_term where
   term_to_ground = gterm_of_term and term_from_ground = term_of_gterm and
   term_is_ground = is_ground
   by unfold_locales
+
+global_interpretation "term": smaller_subterms where
+  subterms = args and size = size and is_var = is_Var
+  by unfold_locales (metis in_set_simps(3) supt.intros(1) supt_size term.exhaust_sel term.sel(3))
 
 end
