thys/First_Order_Clause/Polymorphic_Ground_Context.thy
@@ -1,0 +1,12 @@
+theory Polymorphic_Ground_Context
+  imports
+    Abstract_Context
+    Polymorphic_Ground_Term
+begin
+
+interpretation poly_gcontext: abstract_context where 
+  Fun = PGFun and fun_sym = fun_sym and subterms = args and extra = type_args and 
+  is_var = is_var and size = size
+  by unfold_locales
+
+end
