thys/First_Order_Clause/Polymorphic_Ground_Term.thy
@@ -1,0 +1,23 @@
+theory Polymorphic_Ground_Term
+  imports 
+    IsaFoR_Ground_Term
+    Generic_Term
+begin
+
+datatype ('f, 'tyf) poly_gterm =
+  PGFun (fun_sym: 'f) (type_args: "'tyf gterm list") (args: "('f, 'tyf) poly_gterm list")
+
+interpretation poly_gterm: smaller_subterms where
+  subterms = args and size = size and is_var = "\<lambda>_. False"
+proof unfold_locales
+  fix t t' :: "('f, 'tyf) poly_gterm"
+  assume "t' \<in> set (poly_gterm.args t)" 
+  then show "size t' < size t"
+    by (induction t arbitrary: t') (auto simp: elem_size_size_list_size less_SucI trans_less_add2)
+qed
+
+interpretation poly_gterm: term_interpretation where
+  Fun = PGFun and fun_sym = fun_sym and subterms = args and extra = type_args and is_var = is_var
+  by unfold_locales (auto intro: poly_gterm.exhaust)
+
+end
