thys/Superposition_Calculus/Sorted_Terms_Superposition.thy
@@ -2,7 +2,6 @@ theory Sorted_Terms_Superposition
   imports 
     Superposition
 
-    First_Order_Clause.IsaFoR_Ground_Critical_Pairs
     First_Order_Clause.IsaFoR_Nonground_Clause_With_Equality
     First_Order_Clause.IsaFoR_Nonground_Context
     First_Order_Clause.Sorted_Terms_Typing
@@ -20,6 +19,11 @@ locale sorted_terms_superposition_calculus =
   context_to_set = set2_actxt and hole = \<box> and apply_context = ctxt_apply_term and 
   occurences = occurences and ground_hole = \<box> and apply_ground_context = apply_ground_context and
   compose_ground_context = "(\<circ>\<^sub>c)" and ground_context_map = map_args_actxt and
-  ground_context_to_set = set2_actxt and welltyped = welltyped and term_is_ground = term.is_ground
+  ground_context_to_set = set2_actxt and welltyped = welltyped and
+  term_is_ground = term.is_ground and GFun = "\<lambda>f _. GFun f" and GMore = "\<lambda>f _. More f" and
+  ground_fun_sym\<^sub>c = fun_sym\<^sub>c and ground_extra\<^sub>c = "\<lambda>_. ()" and ground_subterms\<^sub>l = subterms\<^sub>l and
+  ground_subcontext = subcontext and ground_subterms\<^sub>r = subterms\<^sub>r and ground_size = size and
+  ground_hole_position = hole_pos and ground_context_at = context_at\<^sub>G and ground_size\<^sub>c = size and
+  ground_subterms = gargs and ground_fun_sym = groot_sym and ground_extra = "\<lambda>_. ()"
 
 end
